pre-rust updates

SP1Chips/BitwiseChip.lean
@@ -5,6 +5,40 @@ open LeanRV32D.Functions Sail
 
 namespace BitwiseChip
 
+-- def constraints (Main : Vector BabyBear 33) : List SP1Constraint :=
+--   let E0 : BabyBear := Main[30] + Main[31]
+--   let E1 : BabyBear := E0 + Main[32]
+--   let E2 : BabyBear := Main[30] - 1
+--   let E3 : BabyBear := Main[30] * E2
+--   let E4 : BabyBear := Main[31] - 1
+--   let E5 : BabyBear := Main[31] * E4
+--   let E6 : BabyBear := Main[32] - 1
+--   let E7 : BabyBear := Main[32] * E6
+--   let E8 : BabyBear := E1 - 1
+--   let E9 : BabyBear := E1 * E8
+--   let E10 : BabyBear := Main[30] * 2
+--   let E11 : BabyBear := Main[31] * 1
+--   let E12 : BabyBear := E10 + E11
+--   let E13 : BabyBear := Main[32] * 0
+--   let E14 : BabyBear := E12 + E13
+--   let E15 : BabyBear := Main[30] * 3
+--   let E16 : BabyBear := Main[31] * 4
+--   let E17 : BabyBear := E15 + E16
+--   let E18 : BabyBear := Main[32] * 5
+--   let E19 : BabyBear := E17 + E18
+--   let ⟨⟨⟨[E20, E21]⟩, _⟩, CS0⟩ := BitwiseU16Operation.constraints #v[Main[11], Main[12]] #v[Main[17], Main[18]] { a_low_bytes := { low_bytes := #v[Main[22], Main[23]] }, bitwise_operation := { result := #v[Main[26], Main[27], Main[28], Main[29]] }, b_low_bytes := { low_bytes := #v[Main[24], Main[25]] } } E14 E1
+--   let E22 : BabyBear := Main[3] + 4
+--   let CS1 : List SP1Constraint := CPUState.constraints { clk_0_16 := Main[2], clk_16_24 := Main[1], clk_high := Main[0], pc := Main[3] } E22 8 E1
+--   let E23 : BabyBear := Main[1] * 65536
+--   let E24 : BabyBear := Main[2] + E23
+--   let CS2 : List SP1Constraint := ALUTypeReader.constraints Main[0] E24 Main[3] E19 #v[E20, E21] { imm_c := Main[21], op_a := Main[4], op_a_0 := Main[9], op_a_memory := { access_timestamp := { diff_low_limb := Main[8], prev_low := Main[7] }, prev_value := #v[Main[5], Main[6]] }, op_b := Main[10], op_b_memory := { access_timestamp := { diff_low_limb := Main[14], prev_low := Main[13] }, prev_value := #v[Main[11], Main[12]] }, op_c := #v[Main[15], Main[16]], op_c_memory := { access_timestamp := { diff_low_limb := Main[20], prev_low := Main[19] }, prev_value := #v[Main[17], Main[18]] } } E1
+--   [
+--     .assertZero E3,
+--     .assertZero E5,
+--     .assertZero E7,
+--     .assertZero E9
+--   ] ++ CS0 ++ CS1 ++ CS2
+
 def constraints
   (Main : Vector BabyBear 33)
   : Word BabyBear × SP1ConstraintList :=
@@ -32,7 +66,7 @@ def constraints
   let Expr44 := 16384 * Main[1]
   let Expr46 := Expr44 + Main[2]
   let ⟨⟨⟨[Expr40, Expr41]⟩, _⟩, BitwiseU16Operation_constraints⟩ :=
-    BitwiseU16Operation.constraintList
+    BitwiseU16Operation.constraints
       #v[Main[11], Main[12]]
       #v[Main[17], Main[18]]
       { a_low_bytes := { low_bytes := #v[Main[22], Main[23]] }
